% Rudin 6.10
% John Lekberg
% 2016-02-25

\newcommand{\closed}[2]{\left[#1,#2\right]}
\newcommand{\open}[2]{\left(#1,#2\right)}
\newcommand{\openclosed}[2]{\left(#1,#2\right]}
\newcommand{\closedopen}[2]{\left[#1,#2\right)}
\renewcommand{\iff}{\Leftrightarrow\,}
\newcommand{\imply}{\Rightarrow\,}
\newcommand{\riemann}{\mathscr{R}}
\newcommand{\d}{\,\mathrm{d}}

# Statement

Let $p$ and $q$ be positive real numbers such that:

$$
\frac{1}{p} + \frac{1}{q} = 1.
$$

Prove the following statements.

(a) If $u\geq 0$ and $v\geq 0$, then:
$$
uv \leq \frac{u^p}{p} + \frac{v^q}{q}
$$
Equality holds if and only if $u^p = v^q$.
(b) If $f\in\riemann(\alpha)$, $g\in\riemann(\alpha)$, $f\geq 0$, $g\geq 0$, and
$$
\int_a^b f^p \d{\alpha} = 1 = \int_a^b g^q \d{\alpha}
$$
then:
$$
\int_a^b fg \d{\alpha} \leq 1
$$
(c) If $f$ and $g$ are complex functions in $\riemann(\alpha)$, then:
$$
\left|\int_a^b fg\d{\alpha}\right| \leq \left\{\int_a^b |f|^p\d{\alpha}\right\}^{1/p} \left\{\int_a^b |g|^q\d{\alpha}\right\}^{1/q}
$$
This is *Hölder's inequality.*
When $p=q=2$ it is usually called the Schwarz inequality.
(Note that Theorem 1.35 is a very special case of this.)
(d) Show that Hölder's inequality is also true for the "improper" integrals described in Exercises 7 and 8.

# Solution

## Part A

Let's rearrange this inequality:

$$
 uv \leq \frac{u^p}{p} + \frac{v^q}{q} \iff 0 \leq \frac{u^p}{p} + \frac{v^q}{q} - uv
$$

Fix an arbitrary $v$ and let $f$ be a function of $u$, where:

$$
f(u) \equiv \frac{u^p}{p} + \frac{v^q}{q} - uv
$$

Now if we can show that $f \geq 0$, then we will have shown that $uv \leq \frac{u^p}{p} + \frac{v^q}{q}$.
Say $v = 0$, then

$$
f(u) = \frac{u^p}{p}
$$

Because $u, p \geq 0$, we know that $f \geq 0$ if $v = 0$.
If both $u$ and $v$ are zero, then:

$$
f = 0 \geq 0.
$$

Since we have shown the inequality holds if one or both of $u$ and $v$ is $0$, now let's consider the case where $u,v > 0$.
We know that

$$
\begin{align}
  & f(u) = \frac{u^p}{p} + \frac{v^q}{q} - uv \\
  \imply & f'(u) = u^{p-1} - v \\
  \imply & f''(u) = (p - 1)u^{p-1}
\end{align}
$$

If we can show that $f'' > 0$, then we know $f$ is convex.
We can use this convexity to easily prove what we need!
First will will make a small aside:

We know that $p,q > 0$.
But I claim that from the relationship $\frac{1}{p} + \frac{1}{q} = 1$ that we know that $p,q > 1$.
Without loss of generality, say $p \leq 1$.
It follows that $\frac{1}{p} \geq 1$.
Therefore

$$
\begin{align}
  & \frac{1}{p} + \frac{1}{q} = 1 \\
  \iff & \frac{1}{q} = 1 - \frac{1}{p} \\
  \imply & \frac{1}{q} \leq 1 - 1 \\
  \iff & \frac{1}{q} \leq 0
\end{align}
$$

This violates our hypothesis that $p,q > 0$.
Therefore it follows from this contradiction that $p,q > 1$.

Remember that we showed that

$$
f''(u) = (p - 1)u^{p-1}
$$

It follows from $p,q > 1$ and $u,v > 0$ that both $(p-1)$ and $u^{p-1}$ are positive.
Therefore $f'' > 0$ when $u,v > 0$.
This means that $f$ is strictly convex under these conditions, therefore $f$ has a unique minimum.
We can find the critical point if we set $f'(u) = 0$ and solve for $u$.
Therefore:

$$
\begin{align}
  & f'(u) = 0 \\
  \iff & u^{p-1} - v = 0 \\
  \iff & u^{p-1} = v \\
  \iff & u = v^{\frac{1}{p-1}}
\end{align}
$$

So we know that $f$ has a minimum at $u = v^{\frac{1}{p-1}}$.
Once again, we can use the relationship between $p$ and $q$ to simplify $\frac{1}{p-1}$:

$$
\begin{align}
  & \frac{1}{p} + \frac{1}{q} = 1 \\
  \imply & p + q = pq \\
  \imply & \frac{p}{q} + 1 = p \\
  \iff & \frac{p}{q} = p - 1 \\
  \imply & \frac{q}{p} = \frac{1}{p-1}
\end{align}
$$

Therefore we know that $f$ reaches its unique minimum at $u = v^\frac{q}{p}$, which is equivalent to stating that $u^p = v^q$.
What value does $f$ take at this minimum?
Let's find out!

$$
\begin{align}
  & f(v^\frac{q}{p}) = \frac{\left(v^\frac{q}{p}\right)^p}{p} + \frac{v^q}{q} - v^\frac{q}{p}v \\
  \imply & f(v^\frac{q}{p}) = \frac{v^q}{p} + \frac{v^q}{q} - v^{1 + \frac{q}{p}} \\
  \iff & f(v^\frac{q}{p}) = v^q\left(\frac{1}{p} + \frac{1}{q}\right) - v^{1 + \frac{q}{p}} \\
  \imply & f(v^\frac{q}{p}) = v^q - v^{1 + \frac{q}{p}} \\
  \iff & f(v^\frac{q}{p}) = v^q - v^q \\
  \imply & f(v^\frac{q}{p}) = 0
\end{align}
$$

Therefore the minimum value of $f$ is $0$.
So $f \geq 0$ if $u, v > 0$.
Since we also showed that $f \geq 0$ if one or both of $u$ and $v$ is $0$, then for any $u,v \geq 0$:

$$
\begin{align}
  & (u,v > 0 \imply f \geq 0) \land (uv = 0 \imply f \geq 0) \\
  \imply & u,v \geq 0 \imply f \geq 0 \\
\end{align}
$$

Because $f\geq 0$, we have equivalently stated:

$$
uv \leq \frac{u^p}{p} + \frac{v^q}{q}
$$

We also need to show that equality only holds if $u^p = v^q$.
We showed that for all $u,v > 0$, that $f(u) = 0$ if and only if $u^p = v^q$.
Then if one of $u$ and $v$ is $0$ and we know that $u^p = v^q$, then it follows that both $u$ and $v$ equal $0$.
If both $u$ and $v$ equal $0$, then $f = 0$, so it follows that we have equality.

## Part B

By Part A, we know that:

$$
fg \leq \frac{f^p}{p} + \frac{g^q}{q}
$$

Therefore it follows by direct computation that:

$$
\begin{align}
  & fg \leq \frac{f^p}{p} + \frac{g^q}{q} \\
  \imply & \int_a^b fg \d{\alpha} \leq \int_a^b \frac{f^p}{p} \d{\alpha} + \int_a^b \frac{g^q}{q} \d{\alpha} \\
  \iff & \int_a^b fg \d{\alpha} \leq \frac{1}{p}\int_a^b f^p \d{\alpha} + \frac{1}{q} \int_a^b g^q \d{\alpha} \\
  \imply & \int_a^b fg \d{\alpha} \leq \frac{1}{p} + \frac{1}{q} \\
  \imply & \int_a^b fg \d{\alpha} \leq 1
\end{align}
$$

## Part C

Since $f,g\in\riemann(\alpha)$ we know that $\int_a^b f\d{\alpha}$ and $\int_a^b g\d{\alpha}$ exist and are finite.
Say that one or both of $\int_a^b f\d{\alpha}$ and $\int_a^b g\d{\alpha}$ are zero.
Without loss of generality, let's say $\int_a^b f\d{\alpha} = 0$.
This implies that $f = 0$, which means that the inequality we want to prove reduces to:

$$
0 \leq 0
$$

Which is obviously true.
Now assume that $\int_a^b f\d{\alpha}$ and $\int_a^b g\d{\alpha}$ **don't** equal $0$.
We want to use our results from Part B to help us, but we don't have the extra properties of $f$ and $g$ that are required to use Part B.
Let's create auxiliary functions with those properties.
Define $F$ as:

$$
F \equiv \frac{|f|}{\left(\int_a^b |f|^p\d{\alpha}\right)^{1/p}}
$$

and $G$ as:

$$
G \equiv \frac{|g|}{\left(\int_a^b |g|^q\d{\alpha}\right)^{1/p}}
$$

Notice that $F$ and $G$ have the properties that $F, G \geq 0$ and that:

$$
\int_a^b F^p \d{\alpha} = 1 = \int_a^b G^q \d{\alpha}
$$

Therefore, by our results from Part B we know that:

$$
\int_a^b FG\d{\alpha} \leq 1.
$$

Let's see how we can rewrite this:

$$
\begin{align}
  & \int_a^b FG\d{\alpha} \leq 1 \\
  \iff & \int_a^b \frac{|f|}{\left(\int_a^b |f|^p\d{\alpha}\right)^{1/p}} \frac{|g|}{\left(\int_a^b |g|^q\d{\alpha}\right)^{1/p}}} \leq 1 \\
  \imply & \int_a^b |f||g| \d{\alpha} \leq \left(\int_a^b |f|^p\d{\alpha}\right)^{1/p}\left(\int_a^b |g|^q\d{\alpha}\right)^{1/p} \\
  \imply & \left|\int_a^b fg\d{\alpha}\right| \leq \left(\int_a^b |f|^p\d{\alpha}\right)^{1/p}\left(\int_a^b |g|^q\d{\alpha}\right)^{1/p}
\end{align}
$$

We have proved what we set out to!

## Part D

**IN PROGRESS**
