% Rudin 6.11
% John Lekberg
% 2016-02-25

\newcommand{\norm}[1]{\left\lVert #1\right\rVert}
\newcommand{\closed}[2]{\left[#1,#2\right]}
\newcommand{\open}[2]{\left(#1,#2\right)}
\newcommand{\openclosed}[2]{\left(#1,#2\right]}
\newcommand{\closedopen}[2]{\left[#1,#2\right)}
\renewcommand{\iff}{\Leftrightarrow\,}
\newcommand{\imply}{\Rightarrow\,}
\newcommand{\riemann}{\mathscr{R}}
\newcommand{\d}{\,\mathrm{d}}

# Statement

Let $\alpha$ be a fixed increasing function on $\closed{a}{b}$. For $u\in\riemann(\alpha)$, define:

$$
\norm{u}_{2} = \left\{\int_a^b |u|^2 \d{\alpha}\right\}^{1/2}.
$$

Suppose $f,g,h\in\riemann(\alpha)$, and prove the triangle inequality:

$$
\norm{f-h}_{2} \leq \norm{f - g}_2 + \norm{g-h}_2
$$

as a consequence of the Schwarz Inequality, as in the proof of Theorem 1.37.

# Solution

This proof follows the proof of Theorem 1.37 very closely.
First I will show that $\norm{u + v}_2 \leq \norm{u}_2 + \norm{v}_2$ for all $u,v\in\riemann(\alpha)$.

$$
\begin{align}
  & \norm{u+v}_2^2 = \int_a^b |u+v|^2\d{\alpha} \\
  \iff & \norm{u+v}_2^2 = \int_a^b (u+v)^2\d{\alpha} \\
  \iff & \norm{u+v}_2^2 = \int_a^b (u^2 + 2uv + v^2)\d{\alpha} \\
  \iff & \norm{u+v}_2^2 = \int_a^b u^2\d{\alpha} + 2\int_a^b uv\d{\alpha} + \int_a^b v^2 \d{\alpha}\\
  \imply & \norm{u+v}_2^2 \leq \int_a^b |u|^2\d{\alpha} + 2\left|\int_a^b uv\d{\alpha}\right| + \int_a^b |v|^2 \d{\alpha}\\
  \iff & \norm{u+v}_2^2 \leq \norm{u}_2^2 + 2\left|\int_a^b uv\d{\alpha}\right| + \norm{v}_2^2 \\
  \imply & \norm{u+v}_2^2 \leq \norm{u}_2^2 + 2\norm{u}_2 \norm{v}_2 + \norm{v}_2^2 \\
  \iff & \norm{u+v}_2^2 \leq \left(\norm{u}_2 + \norm{v}_2\right)^2 \\
  \imply & \norm{u+v}_2 \leq \norm{u}_2 + \norm{v}_2
\end{align}
$$

This follows because we know that given any $x$,

$$
x \leq |x|
$$

and from Problem 6.10.c, we know that:

$$
\left|\int_a^b fg\right| \leq \norm{f}_2 \norm{g}_2
$$

(This is a special case of HÃ¶lder's inequality.)
Theorem 6.12.a states:

> If $f_1\in\riemann(\alpha)$ and $f_2\in\riemann(\alpha)$ on $\closed{a}{b}$, then
$$
f_1 + f_2 \in\riemann(\alpha)
$$

Therefore by Theorem 6.12.a, $f - g\in\riemann(\alpha)$ and $g - h\in\riemann(\alpha)$.
Therefore we know that:

$$
\norm{f-h}_2 = \norm{f - g + g - h}_2 \leq \norm{f - g}_2 + \norm{g - h}_2
$$

Therefore we have shown the triangle inequality for 2-norms.
