% Rudin 6.17
% John Lekberg

# Statement

Suppose $\alpha$ increases monotonically on $\closed{a}{b}$, $g$ is continuous, and $g(x) = G'(x)$ for $a\leq x \leq b$.
Prove that

$$
\int_a^b \alpha(x)g(x)\d{x} = G(b)\alpha(b) - G(a)\alpha(a) - \int_a^b G\d{\alpha}
$$

*Hint:* Take $g$ real, without loss of generality.
Given $P=\{x_0,x_1,\ldots,x_n\}$, choose $t_i\in(x_{i-1},x_i)$ so that $g(t_i)\Delta x_i = G(x_i) - G(x_{i-1})$.
Show that

$$
\sum_{i=1}^{n}\alpha(x_i)g(t_i)\Delta x_i = G(b)\alpha(b) - G(a)\alpha(a) - \sum_{i=1}^{n}G(x_{i-1})\Delta \alpha_i.
$$

# Solution
