---
author:
  - John Lekberg <jclekberg@gmail.com>
date: 2016-02-19
...

\renewcommand{\iff}{\Leftrightarrow\,}
\newcommand{\imply}{\Rightarrow\,}
\newcommand{\lowerint}{\underline{\int}}
\newcommand{\upperint}{\overline{\int}}
\newcommand{\d}{\,\mathrm{d}}

# Statement

Suppose $f\geq 0$, $f$ is continuous on $[a,b]$, and $\int_a^b f(x)\d{x} = 0$.
Prove that $f(x) = 0$ for all $x\in[a,b]$.
(Compare this with Exercise 1.)

# Solution

We will prove this by contradiction.
Say that there exists some $x_0\in[a,b]$ where $f(x_0) \neq 0$.
Because $f$ is continuous, pick $\epsilon < |f(x_0)|$.
We get a $\delta > 0$ where for all $x\in(x_0 - \delta, x_0 + \delta)$ we know that:

$$
\begin{align}
 & |f(x_0) - f(x)| < \epsilon \\
 \iff & -\epsilon < f(x_0) - f(x) < \epsilon \\
 \iff & -\epsilon - f(x_0) < - f(x) < \epsilon - f(x_0) \\
 \iff & \epsilon + f(x_0) > f(x) > f(x_0) - \epsilon \\
 \iff & f(x_0) - \epsilon < f(x) < \epsilon + f(x_0) \\
 \iff &f(x_0) - \epsilon < f(x) < f(x_0) + \epsilon
\end{align}
$$

If $f(x_0) < 0$, then we see that

$$
f(x) < 0, x\in(x_0 - \delta, x_0 + \delta)
$$

and if $f(x_0) > 0$, then we see that

$$
f(x) > 0, x\in(x_0 - \delta, x_0 + \delta)
$$

Take some $[c,d]\subset(x_0 - \delta, x_0 + \delta)$.
Any partition $P$ can be refined to $P^{\star}$, where $\{c,d\}\subset P^{\star}$.

If $f(x_0) > 0$, then we know that $M_i > 0$ for all $x_i$ and $x_{i+1}$ in $[c,d]$.
Therefore $\upperint_{a}^{b}f(x)\d{x} \neq 0$.

If $f(x_0) < 0$, then we know that $m_i < 0$ for all $x_i$ and $x_{i+1}$ in $[c,d]$.
Therefore $\lowerint_{a}^{b}f(x)\d{x} \neq 0$.

However, we know that $\int_a^b f(x)dx = 0$.
Therefore:

$$
\begin{align}
 & \int_a^b f(x)\d{x} = 0 \\
 \iff & \lowerint_a^b f(x)\d{x} = \upperint_a^b f(x)\d{x} = 0 \\
 \iff & \lowerint_a^b f(x)\d{x} = 0 \land \upperint_a^b f(x)\d{x} = 0
\end{align}
$$

We showed that at least one of $\lowerint_a^b f(x)\d{x} = 0$ and $\upperint_a^b f(x)\d{x} = 0$ is false.
Therefore, $\int_a^b f(x)\d{x} \neq 0$.
This contradicts our assumptions, therefore $\forall x,f(x) = 0$.
