% Rudin 6.3
% John Lekberg
% 2016-02-20

\renewcommand{\iff}{\Leftrightarrow\,}
\newcommand{\imply}{\Rightarrow\,}
\newcommand{\lowerint}{\underline{\int}}
\newcommand{\upperint}{\overline{\int}}
\newcommand{\d}{\,\mathrm{d}}
\newcommand{\riemann}{\mathscr{R}}

# Statement

Define three functions $\beta_1$, $\beta_2$, $\beta_3$ as follows: $\beta_j(x) = 0$ if $x < 0$, $\beta_j(x) = 1$ if $x > 0$ for $j = 1,2,3$; and $\beta_1(0) = 0$, $\beta_2(0) = 1$ and $\beta_3(0) = \frac{1}{2}$.
Let $f$ be a bounded function on $[-1,1]$.

a. Prove that $f\in\riemann(\beta_1)$ if and only if $f(0+) = f(0)$ and that then $$\int f\d{\beta_1}=f(0).$$
b. State and prove a similar result for $\beta_2$.
c. Prove that $f\in\riemann(\beta_3)$ if and only if $f$ is continuous at $0$.
d. If $f$ is continuous at $0$ prove that $$
\int f\d{\beta_1} = \int f\d{\beta_2} = \int f\d{\beta_3} = f(0)
$$

# Solution

## Part A

First I will prove that

$$
f(0+) \neq f(0) \implies f\not\in\riemann(\beta_1)
$$

Take any partition $P$.
There exists some $1\leq j \leq n$ where:

$$
x_{j-1} \leq 0 < x_{j}
$$

Now I will show you how we can compute the difference between the lower and upper sums.
First let's find $U(P,f,\beta_1)$:

$$
\begin{align}
  & U(P,f,\beta_1) = \sum_{i=1}^{n}M_i\Delta\beta_{1,i} \\
  \iff & U(P,f,\beta_1) = \sum_{i=1}^{j-1}M_i\Delta\beta_{1,i} + M_j\Delta\beta_{1,j} + \sum_{i=j+1}^{n}M_i\Delta\beta_{1,i}
\end{align}
$$

I claim that $\sum_{i=1}^{j-1}M_i\Delta\beta_{1,i} = 0$.
It follows by the definition of $\beta_1$ as:

$$
\beta_1(x) = \begin{cases}
  0, & x \leq 0 \\
  1, & x > 0
\end{cases}
$$

and that if $i < j$ then $x_i \leq 0$, then:

$$
\begin{align}
  & \sum_{i=1}^{j-1}M_i\Delta\beta_{1,i} = \sum_{i=1}^{j-1}M_i(\beta_1(x_i) - \beta_1(x_{i-1})) \\
  \imply & \sum_{i=1}^{j-1}M_i\Delta\beta_{1,i} = \sum_{i=1}^{j-1}M_i(0 - 0) \\
  \iff & \sum_{i=1}^{j-1}M_i\Delta\beta_{1,i} = 0
\end{align}
$$

Now I claim that $\sum_{i=j+1}^{n}M_i\Delta\beta_{1,i} = 0$.
If follows from the definition of $\beta_1$ and the fact that if $i \geq j$ then $x_i > 0$, that:

$$
\begin{align}
  & \sum_{i=j+1}^{n}M_i\Delta\beta_{1,i} = \sum_{i=j+1}^{n}M_i(\beta_1(x_i) - \beta_1(x_{i-1})) \\
  \imply & \sum_{i=j+1}^{n}M_i\Delta\beta_{1,i} = \sum_{i=j+1}^{n}M_i(1 - 1) \\
  \iff & \sum_{i=j+1}^{n}M_i\Delta\beta_{1,i} = 0
\end{align}
$$

Therefore we can go back to our original computation:

$$
\begin{align}
  & U(P,f,\beta_1) = \sum_{i=1}^{j-1}M_i\Delta\beta_{1,i} + M_j\Delta\beta_{1,j} + \sum_{i=j+1}^{n}M_i\Delta\beta_{1,i} \\
  \imply & U(P,f,\beta_1) = M_j\Delta\beta_{1,j} \\
  \iff & U(P,f,\beta_1) = M_j(\beta_1(x_j) - \beta(x_{j-1})) \\
  \imply & U(P,f,\beta_1) = M_j(1 - 0) \\
  \iff & U(P,f,\beta_1) = M_j
\end{align}
$$

We can use the same process to prove $L(P,f,\beta_1) = m_j$.
(I have omitted the calculations for this.)
Therefore, we know that for any partition $P$:

$$
U(P,f,\beta_1) - L(P,f,\beta_1) = M_j - m_j
$$

Where $1 \leq j \leq n$ such that $x_{j-1} \leq 0 < x_{j}$.

Theorem 6.6 states that:

> $f\in\riemann(\alpha)$ on $[a,b]$ if and only if for every $\epsilon > 0$ there exists a partition $P$ such that
$$
U(P,f,\alpha) - L(P,f,\alpha) < \epsilon
$$

So to show that $f\not\in\riemann(\beta_1)$, we need to show that there exists an $\epsilon > 0$ such that for every partition $P$:
$$
U(P,f,\beta_1) - L(P,f,\beta_1) > \epsilon
$$

We have assumed that $f(0+) \neq f(0)$.
We know that because $f$ is bounded $f(0+)$ exists, so let's define $c\equiv f(0+)$.
We know that $c < f(0)$ or $f(0) > c$.
I claim that $M_j \geq \max\{c,f(0)\}$ and $m_j \leq \min\{c,f(0)\}$.

It is obvious that $M_j > f(0)$ and $m_j < f(0)$, but say $M_j < c$ or $m_j > c$ then we can find an $x\in[x_{j-1},x_{j}]$ where $f(x)$ is less than $\min\{|c - M_j|, |c - m_j|\}$ from $c$.
This violates the supremum and infimum properties of $M_j$ and $m_j$, therefore $M_j \geq c$ and $m_j \leq c$.

From this we know that:

$$
\begin{align}
  & M_j \geq \max\{c,f(0)\} \land m_j \leq \min\{c,f(0)\} \\
  \imply & M_j - m_j \geq \max\{c,f(0)\} - \min\{c,f(0)\} \\
  \iff & M_j - m_j \geq |\max\{c,f(0)\} - \min\{c,f(0)\}| \\ \\
  \iff & M_j - m_j \geq |c - f(0)| > 0 \\
  \imply & M_j - m_j > \frac{|c - f(0)|}{2}
\end{align}
$$

Because this holds for any partition $P$, if we take $\epsilon \equiv \frac{|c - f(0)|}{2}$, then by the contrapositive to Theorem 6.6 $f\not\in\riemann(\beta_1)$.
So we have proved that:

$$
f(0+) \neq f(0) \implies f\not\in\riemann(\beta_1)
$$

Now I will prove that:

$$
f(0+) = f(0) \implies f\in\riemann(\beta_1)
$$

From earlier calculations, I showed that for any partition $P$:

$$
U(P,f,\beta_1) - L(P,f,\beta_1) = M_j - m_j
$$

Where $1 \leq j \leq n$ such that $x_{j-1} \leq 0 < x_{j}$.

Fix an arbitrary $\epsilon > 0$.
Because $f(0+) = f(0)$ we can find a $\delta > 0$ such that:

$$
\forall x\in[0,\delta], |f(0) - f(x)| < \frac{\epsilon}{3}
$$

Create an arbitrary partition $P$ where $x_j = \delta$ and $x_{j-1} = 0$.
Then by the supremum property $M_j \leq f(0) + \frac{\epsilon}{3}$ and by the infimum property $m_j \geq f(0) - \frac{\epsilon}{3}$.
Using our inequality from earlier, we get:

$$
\begin{align}
  & U(P,f,\beta_1) - L(P,f,\beta_1) = M_j - m_j \\
  \imply & U(P,f,\beta_1) - L(P,f,\beta_1) \leq (f(0) + \frac{\epsilon}{3}) - (f(0) - \frac{\epsilon}{3}) \\
  \imply & U(P,f,\beta_1) - L(P,f,\beta_1) \leq \frac{2}{3}\epsilon \\
  \imply & U(P,f,\beta_1) - L(P,f,\beta_1) < \epsilon
\end{align}
$$

Because $\epsilon$ is arbitrary, then for any $\epsilon > 0$, there exists a partition $P$ such that

$$
U(P,f,\beta_1) - L(P,f,\beta_1) < \epsilon
$$

Therefore, by Theorem 6.6 $f\in\riemann(\beta_1)$.
Thus, we have proven:

$$
\begin{align}
  & f(0+) = f(0) \imply f\in\riemann(\beta_1) \land f(0+) \neq f(0) \imply f\not\in\riemann(\beta_1) \\
  \imply & f(0+) = f(0) \iff f\in\riemann(\beta_1)
\end{align}
$$

To finish this part, we have to show that $$\int f\d{\beta_1} = 0.$$
From our earlier calculations, we showed that given any $\epsilon > 0$ there exists a partition $P$ where $x_j = \delta$ and $x_{j-1} = 0$, where $\forall x\in[0,\delta]$,

$$
|f(0) - f(x)| < \frac{\epsilon}{3}
$$

Therefore $0 \leq M_j - f(0) < \epsilon$, because $M_j \geq f(0)$ by the supremum property.
Because this holds for any $\epsilon > 0$, we know that:

$$
\begin{align}
  & \inf U(P,f,\beta_1) = f(0) \\
  \iff & \lowerint f\d{\beta_1} = f(0)
\end{align}
$$

Because we know that $f\in\riemann(\beta_1)$, then

$$
\int f\d{\beta_1} = \upperint f\d{\beta_1} = \lowerint f\d{\beta_1}
$$

Therefore:

$$
\begin{align}
   & \lowerint f\d{\beta_1} = f(0) \\
   \imply & \int f\d{\beta_1} = f(0)
\end{align}
$$

There we have shown that

$$
f(0+) = f(0) \iff f\in\riemann(\beta_1)
$$

and that if $f\in\riemann(\beta_1)$, then:

$$
\int f\d{\beta_1} = f(0)
$$

## Part B

We want to prove that

$$
f(0-) = f(0) \iff f\in\riemann(\beta_2)
$$

and that if $f\in\riemann(\beta_2)$, then:

$$
\int f\d{\beta_2} = f(0).
$$

First I will prove that:

$$
f(0-) \neq f(0) \imply f\not\in\riemann(\beta_2)
$$

Take any partition $P$.
There exist some $1\leq j \leq n$ where:

$$
x_{j-1} < 0 \leq x_{j}$
$$

Now we will compute the different between the lower and upper sums.
Using the same process as in Part A:

$$
U(P,f,\beta_2) = \sum_{i=1}^{j-1}M_i\Delta\beta_{2,i} + M_j\Delta\beta_{2,j} + \sum_{i=j+1}^{n}M_i\Delta\beta_{2,i}
$$

From the definition of $\beta_2$:

$$
\beta_2(x) = \begin{cases}
  0, & x < 0 \\
  1, & x \geq 0
\end{cases}
$$

We can show that $\sum_{i=1}^{j-1}M_i\Delta\beta_{2,i} = 0$ and $\sum_{i=j+1}^{n}M_i\Delta\beta_{2,i} = 0$.
(This uses the same process as in Part A.)
Therefore we know that

$$
\begin{align}
  & U(P,f,\beta_2) = \sum_{i=1}^{j-1}M_i\Delta\beta_{2,i} + M_j\Delta\beta_{2,j} + \sum_{i=j+1}^{n}M_i\Delta\beta_{1,i}
  \imply & U(P,f,\beta_2) = M_j\Delta\beta_{2,j} \\
  \iff & U(P,f,\beta_2) = M_j(\beta_2(x_j) - \beta_2(x_{j-1})) \\
  \imply & U(P,f,\beta_2) = M_j(1 - 0) \\
  \iff & U(P,f,\beta_2) = M_j
\end{align}
$$

Likewise, we can prove that $L(P,f,\beta_2) = m_j$.
(I have omitted the calculations for this.)
Therefore, for any partition $P$:

$$
U(P,f,\beta_1) - L(P,f,\beta_1) = M_j - m_j
$$

Where $1 \leq j \leq n$ such that $x_{j-1} \leq 0 < x_{j}$.

Theorem 6.6 states that:

> $f\in\riemann(\alpha)$ on $[a,b]$ if and only if for every $\epsilon > 0$ there exists a partition $P$ such that
$$
U(P,f,\alpha) - L(P,f,\alpha) < \epsilon
$$

So to show that $f\not\in\riemann(\beta_2)$, we need to show that there exists an $\epsilon > 0$ such that for every partition $P$:
$$
U(P,f,\beta_2) - L(P,f,\beta_2) > \epsilon
$$

We have assumed that $f(0-) \neq f(0)$.
Because $f$ is bounded, hten $f(0-)$ exists, so let's define $c\equiv f(0-)$.
We know that $c < f(0)$ or $f(0) > c$.
Like Part A, I claim that $M_j \geq \max\{c,f(0)\}$ and $m_j \leq \min\{c,f(0)\}$.

From this we know that:

$$
\begin{align}
  & M_j \geq \max\{c,f(0)\} \land m_j \leq \min\{c,f(0)\} \\
  \imply & M_j - m_j > \frac{|c - f(0)|}{2}
\end{align}
$$

Because this holds for any partition $P$, if we take $\epsilon \equiv \frac{|c - f(0)|}{2}$, then by the contrapositive to Theorem 6.6 $f\not\in\riemann(\beta_2)$.
So we have proved that:

$$
f(0-) \neq f(0) \implies f\not\in\riemann(\beta_2)
$$

Now I will prove that:

$$
f(0-) = f(0) \implies f\in\riemann(\beta_2)
$$

From above, I showed that for any parition $P$:

$$
U(P,f,\beta_2) - L(P,f,\beta_2) = M_j - m_j
$$

Where $1 \leq j \leq n$ such that $x_{j-1} \leq 0 < x_{j}$.

Fix an arbitrary $\epsilon > 0$.
Because $f(0-) = f(0)$ we can find a $\delta > 0$ such that

$$
\forall x\in[-\delta,0], |f(0) - f(x)| < \frac{\epsilon}{3}
$$

Create an arbitrayr partition $P$ where $x_j = 0$ and $x_{j-1} = -\delta$.
Then by the supremum property $M_j \leq f(0) + \frac{\epsilon}{3}$ and by the infimum property $m_j \geq f(0) + \frac{\epsilon}{3}$.
Using our inequality from earlier, we get:

$$
\begin{align}
  & U(P,f,\beta_2) - L(P,f,\beta_2) = M_j - m_j \\
  \imply & U(P,f,\beta_2) - L(P,f,\beta_2) \leq (f(0) + \frac{\epsilon}{3}) - (f(0) - \frac{\epsilon}{3}) \\
  \imply & U(P,f,\beta_2) - L(P,f,\beta_2) \leq \frac{2}{3}\epsilon \\
  \imply & U(P,f,\beta_2) - L(P,f,\beta_2) < \epsilon
\end{align}
$$

Because $\epsilon$ is arbitrary, then for any $\epsilon > 0$, there exists a partition $P$ such that:

$$
U(P,f,\beta_2) - L(P,f,\beta_2) < \epsilon
$$


Therefore, by Theorem 6.6, $f\in\riemann(\beta_2).
Thus, we have proven:

$$
\begin{align}
  & f(0-) = f(0) \imply f\in\riemann(\beta_2) \land f(0+) \neq f(0) \imply f\not\in\riemann(\beta_2) \\
  \imply & f(0-) = f(0) \iff f\in\riemann(\beta_2)
\end{align}
$$

To finish this part, we have to show that $$\int f\d{\beta_2} = 0.$$
From our earlier calculations, we showed that given any $\epsilon > 0$, there exists a partition $P$ where $x_j = 0$ and $x_{j-1} = -\delta$, where $\forall x\in[-\delta,0]$

$$
|f(0) - f(x)| < \frac{\epsilon}{3}
$$

Therefore $0 \leq M_j - f(0) < \epsilon$, because $M_j \geq f(0)$ by the supremum property.
Because this holds for any $\epsilon > 0$, we know that:

$$
\begin{align}
  & \inf U(P,f,\beta_2) = f(0) \\
  \iff & \lowerint f\d{\beta_2} = f(0)
\end{align}
$$

Because we know that $f\in\riemann(\beta_2)$, then

$$
\int f\d{\beta_2} = \upperint f\d{\beta_2} = \lowerint f\d{\beta_2}
$$

Therefore:

$$
\begin{align}
   & \lowerint f\d{\beta_2} = f(0) \\
   \imply & \int f\d{\beta_2} = f(0)
\end{align}
$$

There we have shown that

$$
f(0-) = f(0) \iff f\in\riemann(\beta_2)
$$

and that if $f\in\riemann(\beta_2)$, then:

$$
\int f\d{\beta_2} = f(0)
$$

## Part C

First I will prove that:

$$
\lim_{x\to 0}f(x) \neq f(0) \imply f\not\in\riemann(\beta_3)
$$

If we know that $\lim_{x\to0}f(x) \neq f(0)$ then we know that $f(0+) \neq f(0)$ and $f(0-) \neq f(0)$.
Take any partition $P$ where there exists $x_j = 0$.
First let's find $U(P,f,\beta_3)$:

$$
\begin{align}
  & U(P,f,\beta_3) = \sum_{i=1}^{n}M_i\Delta\beta_{3,i} \\
  \iff & U(P,f,\beta_3) = \sum_{i=1}^{j-1}M_i\Delta\beta_{3,i} + M_j\Delta\beta_{3,j} + M_{j+1}\Delta\beta_{3,j+1} + \sum_{i=j+2}^{n}M_i\Delta\beta_{3,i}
\end{align}
$$

By the methods used in Parts A and B, we can show that $\sum_{i=1}^{j-1}M_i\Delta\beta_{3,i} = 0$ and $\sum_{i=j+2}^{n}M_i\Delta\beta_{3,i} = 0$.
Therefore we can rewrite the above as:

$$
\begin{align}
  & U(P,f,\beta_3) = \sum_{i=1}^{j-1}M_i\Delta\beta_{3,i} + M_j\Delta\beta_{3,j} + M_{j+1}\Delta\beta_{3,j+1} + \sum_{i=j+2}^{n}M_i\Delta\beta_{3,i} \\
  \imply & U(P,f,\beta_3) = M_j\Delta\beta_{3,j} + M_{j+1}\Delta\beta_{3,j+1} \\
  \iff & U(P,f,\beta_3) = M_j(\beta_3(x_j) - \beta_3(x_{j-1})) + M_{j+1}(\beta_3(x_{j+1}) - beta_3(x_j)) \\
  \imply & U(P,f,\beta_3) = M_j\left(\frac{1}{2} - 0\right) + M_{j+1}\left(1 - \frac{1}{2}\right) \\
  \iff & U(P,f,\beta_3) = \frac{M_j + M_{j+1}}{2}
\end{align}
$$

We can use the same process to prove $L(P,f,\beta_3) = \frac{m_j + m_{j+1}}{2}$.
(I have omitted the calculations for this.)
Therefore, we know that for any partition $P$ where $x_j = 0$:

$$
\begin{align}
  & U(P,f,\beta_3) - L(P,f,\beta_3) = \frac{M_j + M_{j+1}}{2} - \frac{m_j + m_{j+1}}{2} \\
  \iff & U(P,f,\beta_3) - L(P,f,\beta_3) = \frac{M_j - m_j}{2} + \frac{M_{j+1} - m_{j+1}}{2} \\
  \imply & U(P,f,\beta_3) - L(P,f,\beta_3) \leq \frac{M_j - m_j}{2} + \frac{M_{j+1} - m_{j+1}}{2}
\end{align}
$$

Notice that we have the restriction that $P$ has an $x_j = 0$.
Theorem 6.4 states:

> If $P^{\star}$ is a refinement of $P$, then
$$
  L(P,f,\alpha) \leq L(P^{\star},f,\alpha)
$$
and
$$
  U(P,f,\alpha) \geq L(P^{\star},f,\alpha)
$$

Therefore for any partition $P$, we can refine it to $P^{\star}$ which includes $x_j = 0$, where:

$$
\begin{align}
  & U(P^{\star},f,\beta_3) - L(P^{\star},f,\beta_3) \leq \frac{M_j - m_j}{2} + \frac{M_{j+1} - m_{j+1}}{2} \\
  \imply & U(P,f,\beta_3) - L(P,f,\beta_3) \leq U(P^{\star},f,\beta_3) - L(P^{\star},f,\beta_3) \leq \frac{M_j - m_j}{2} + \frac{M_{j+1} - m_{j+1}}{2} \\
  \imply & U(P,f,\beta_3) - L(P,f,\beta_3) \leq \frac{M_j - m_j}{2} + \frac{M_{j+1} - m_{j+1}}{2} \\
\end{align}
$$

Therefore this holds for any partition $P$.
Theorem 6.6 states that:

> $f\in\riemann(\alpha)$ on $[a,b]$ if and only if for every $\epsilon > 0$ there exists a partition $P$ such that
$$
U(P,f,\alpha) - L(P,f,\alpha) < \epsilon
$$

So to show that $f\not\in\riemann(\beta_3)$, we need to show that there exists an $\epsilon > 0$ such that for every partition $P$:
$$
U(P,f,\beta_3) - L(P,f,\beta_3) > \epsilon
$$

We have assumed that $f(0+) \neq f(0)$ and $f(0-) \neq f(0)$.
Because $f$ is bounded, both $f(0+)$ and $f(0-)$ exist.
Define $c\equiv f(0+)$ and $c'\equiv f(0-)$.
I claim that $M_j \geq \max\{c, f(0)\}$, $m_j \leq \min\{c,f(0)\}$, $M_{j+1} \geq \max\{c', f(0)\}$ and $m_{j+1} \leq \min\{c', f(0)\}$ using the same reasoning as in Parts A and B.
(AKA, if this is not true, then the supremum and infimum properties are violated.)

Using similar reasoning as in Parts A and be we can deduce that

$$
M_j - m_j > \frac{|c - f(0)|}{2}
$$

and that:

$$
M_{j+1} - m_{j+1} > \frac{|c' - f(0)|}{2}
$$

Because this holds for any partition $P$, if we take $\epsilon \equiv \frac{|c - f(0)| + |c' - f(0)|}{4}$, then by the contrapositive to THeorem 6.6 $f\not\in\riemann(\beta_3)$.
So we have proved that:

$$
\lim_{x\to0}f(x) \neq 0 \implies f\not\in\riemann(\beta_3)
$$

Now I will prove that:

$$
\lim_{x\to0}f(x) = f(0) \implies f\in\riemann(\beta_3)
$$

From earlier calculations, I showed that for any partition $P$:

$$
U(P,f,\beta_3) - L(P,f,\beta_3) \leq \frac{M_j - m_j}{2} + \frac{M_{j+1} - m_{j+1}}{2}
$$

Where $P$ can be refined to have $x_j = 0$.

Fix an arbitrary $\epsilon > 0$.
Because $\lim_{x\to 0}f(x) = f(0)$ we can find a $\delta > 0$ such that:

$$
\forall x\in[-\delta,\delta], |f(0) - f(x)| < \frac{\epsilon}{3}
$$

Take any partition $P$ where $P$ can be refined to have $x_j = 0$.
By the supremum property $M_j \leq f(0) + \frac{\epsilon}{3}$ and $M_{j+1} \leq f(0) + \frac{\epsilon}{3}$.
By the infimum property $m_j \geq f(0) - \frac{\epsilon}{3}$ and $m_{j+1} \leq f(0) - \frac{\epsilon}{3}$.
Using our inequality from earlier, get get:

$$
\begin{align}
  & U(P,f,\beta_3) - L(P,f,\beta_3) \leq \frac{M_j - m_j}{2} + \frac{M_{j+1} - m_{j+1}}{2} \\
  \imply & U(P,f,\beta_3) - L(P,f,\beta_3) \leq \frac{f(0) + \frac{\epsilon}{3}) - (f(0) - \frac{\epsilon}{3}}{2} + \frac{f(0) + \frac{\epsilon}{3}) - (f(0) - \frac{\epsilon}{3}}{2} \\
  \imply & U(P,f,\beta_3) - L(P,f,\beta_3) \leq \frac{2}{3}\epsilon \\
  \imply & U(P,f,\beta_3) - L(P,f,\beta_3) < \epsilon
\end{align}
$$

Because $\epsilon$ is arbitrary, then for any $\epsilon > 0$, there exists a partition $P$ such taht:

$$
U(P,f,\beta_3) - L(P,f,\beta_3) < \epsilon
$$

Therefore, by Theorem 6.6 $f\in\riemann(\beta_3)$.
Thus, we have proven:

$$
\begin{align}
  & \lim_{x\to0}f(x) = f(0) \imply f\in\riemann(\beta_3) \land \lim_{x\to0}f(x) \neq f(0) \imply f\not\in\riemann(\beta_3) \\
  \imply & f(0+) = f(0) \iff f\in\riemann(\beta_3)
\end{align}
$$

## Part D

In Part $C$ we showed that $\forall x\in[-\delta,\delta]$:

$$
|f(0) - f(x)| < \frac{\epsilon}{3}
$$

(We use the fact $\lim_{x\to 0}f(x) = f(0)$ to find such a $\delta$.)
Therefore $0 \leq M_j - f(0) < \epsilon$ and $0 \leq M_{j+1} - f(0) < \epsilon$, because $M_j$ and $M_{j+1}$ are greater than $f(0)$ by the supremum property.
Because this holds for any $\epsilon > 0$, we know taht:

$$
\begin{align}
  & \inf U(P,f,\beta_3) = f(0) \\
  \iff & \lowerint f\d{\beta_3} = f(0)
\end{align}
$$

Because we know that $f\in\riemann(\beta_3)$, then:

$$
\int f\d{\beta_3} = \upperint f\d{\beta_3} = \lowerint f\d{\beta_3}
$$

$$
\begin{align}
   & \lowerint f\d{\beta_3} = f(0) \\
   \imply & \int f\d{\beta_3} = f(0)
\end{align}
$$

This shows that if $f\in\riemann(\beta_3)$, then:

$$
\int f\d{\beta_3} = f(0)
$$

If $f$ is continuous at zero then $\lim_{x\to0}f(x) = f(0)$ and more specifically $f(0+) = f(0)$ and $f(0-) = 0$.
Therefore, by Parts A, B and C:

$$
  \int f\d{\beta_1} = \int f\d{\beta_2} = \int f\d{\beta_3} = 0
$$
