---
author:
  - John Lekberg <jclekberg@gmail.com>
date: 2016-02-21
...

\newcommand{\closed}[2]{\left[#1,#2\right]}
\newcommand{\open}[2]{\left(#1,#2\right)}
\newcommand{\openclosed}[2]{\left(#1,#2\right]}
\newcommand{\closedopen}[2]{\left[#1,#2\right)}
\renewcommand{\iff}{\Leftrightarrow\,}
\newcommand{\imply}{\Rightarrow\,}
\newcommand{\riemann}{\mathscr{R}}
\newcommand{\d}{\,\mathrm{d}}

# Statement

Suppose $f$ is a real function on $(0,1]$ and $f\in\riemann$ on $[c,1]$ for every $c > 0$.
Define

$$
  \int_0^1 f(x)\d{x} = \lim_{c\to0}\int_c^1 f(x)\d{x}
$$

if this limit exists (and is finite).

(a) If $f\in\riemann$ on$[0,1]$, show that this definition of the integral agrees with the old one.
(b) Construct a function $f$ such that the above limit exists, although it fails to exist with $|f|$ in place of $f$.

# Solution

## Part A

Theorem 6.12.c states:

> If $f\in\riemann(\alpha)$ on $\closed{a}{b}$ and if $a < c < b$, then $f\in\riemann(\alpha)$ on $\closed{a}{c}$ and on $\closed{c}{d}$, and
$$
\int_{a}^{c}f\d{\alpha} + \int_{c}^{b}f\d{\alpha} = \int_{a}^{b}f\d{\alpha}
$$

By Theorem 6.12.c, for any $c\in\open{0}{1}$ it follows that:

$$
\begin{align}
  & \int_{0}^{1}f(x)\d{x} = \int_{0}^{c}f(x)\d{x} + \int_{c}^{1}f(x)\d{x} \\
  \iff & \int_{0}^{1}f(x)\d{x} - \int_{c}^{1}f(x)\d{x} = \int_{0}^{c}f(x)\d{x} \\
  \imply & \left|\int_{0}^{1}f(x)\d{x} - \int_{c}^{1}f(x)\d{x}\right| = \left|\int_{0}^{c}f(x)\d{x}\right|
\end{align}
$$

Because $f\in\riemann$ on $\closed{0}{1}$, then it is bounded on $\closed{0}{1}$.
(Rudin himself asserts this in the proof of Theorem 6.20.)
Let $$M\equiv \sup_{x\in\closed{0}{1}} |f(x)|.$$

Theorem 6.12.d states:

> If $f\in\riemann(\alpha)$ on $\closed{a}{b}$ and if $|f(x)| \leq M$ on $\closed{a}{b}$, then
$$
  \left|\int_{a}^{b}f\d{\alpha}\right| \leq M[\alpha(b) - \alpha(a)].
$$

Then by Theorem 6.12.d, it follows that:

$$
\begin{align}
  & \left|\int_{0}^{1}f(x)\d{x} - \int_{c}^{1}f(x)\d{x}\right| = \left|\int_{0}^{c}f(x)\d{x}\right| \\
  \imply & \left|\int_{0}^{1}f(x)\d{x} - \int_{c}^{1}f(x)\d{x}\right| \leq Mc
\end{align}
$$

Because this holds for any $c\in\open{0}{1}$ we can take the limit as $c$ goes to $0$, and we get:

$$
\begin{align}
  & \left|\int_{0}^{1}f(x)\d{x} - \int_{c}^{1}f(x)\d{x}\right| \leq Mc \\
  \imply & \lim_{c\to0^+} \left|\int_{0}^{1}f(x)\d{x} - \int_{c}^{1}f(x)\d{x}\right| \leq \lim_{c\to0^+} Mc \\
  \imply & \left|\int_{0}^{1}f(x)\d{x} - \lim_{c\to0^+}\int_{c}^{1}f(x)\d{x}\right| \leq 0 \\
  \imply & \int_{0}^{1}f(x)\d{x} - \lim_{c\to0^+}\int_{c}^{1}f(x)\d{x} = 0 \\
  \iff & \int_{0}^{1}f(x)\d{x} = lim_{c\to0^+}\int_{c}^{1}f(x)\d{x}
\end{align}
$$

Therefore, if $f\in\riemann$ on $\closed{0}{1}$, then this definition of the integral agrees with the old one.

## Part B

Define the value of the function $f$ at a point $x\in\open{0}{1}$

$$
f\left(\frac{1}{n+1} < x \leq \frac{1}{n}\right) = (-1)^{n+1}(n+1)
$$

Where $n\in\mathbb{N}$.
Then for any $c\in\open{0}{1}$ where there exists $n\in\mathbb{N}$ where $\frac{1}{n+1} < c \leq \frac{1}{n}$, then:

$$
\int_{c}^{1} f(x)\d{x} = \left(\frac{1}{n} - c\right)(-1)^{n+1}(n+1) + \sum_{i=1}^{n-1}(-1)^{i+1}(i+1)\left(\frac{1}{i} - \frac{1}{i+1}\right)
$$

We can simplify this to get it into a useful form:

$$
\begin{align}
  & \int_{c}^{1} f(x)\d{x} = \left(\frac{1}{n} - c\right)(-1)^{n+1}(n+1) + \sum_{i=1}^{n-1}(-1)^{i+1}(i+1)\left(\frac{1}{i} - \frac{1}{i+1}\right) \\
  \iff & \int_{c}^{1} f(x)\d{x} = \left(\frac{1}{n} - c\right)(-1)^{n+1}(n+1) + \sum_{i=1}^{n-1}(-1)^{i+1}(i+1)\left(\frac{1}{i(i+1)}\right) \\
  \iff & \int_{c}^{1} f(x)\d{x} = \left(\frac{1}{n} - c\right)(-1)^{n+1}(n+1) + \sum_{i=1}^{n-1}\frac{(-1)^{i+1}}{i} \\
  \imply & \lim_{c\to0^+}\int_{c}^{1} f(x)\d{x} = \lim_{c\to0^+}\left(\left(\frac{1}{n} - c\right)(-1)^{n+1}(n+1) + \sum_{i=1}^{n-1}\frac{(-1)^{i+1}}{i}\right) \\
\end{align}
$$

Notice that as $c\to0^+$ that $n\to\infty$.
Therefore we can show that:

$$
\begin{align}
  & \left(\frac{1}{n} - \frac{1}{n}\right)(n+1) \leq \left(\frac{1}{n} - c\right)(n+1) \leq \left(\frac{1}{n} - \frac{1}{n+1}\right)(n+1) \\
  \imply & 0 \leq \left(\frac{1}{n} - c\right)(n+1) \leq \left(\frac{1}{n} - \frac{1}{n+1}\right)(n+1) \\
  \iff & 0 \leq \left(\frac{1}{n} - c\right)(n+1) \leq \frac{1}{n} \\
\end{align}
$$

Therefore as $n\to\infty$, then $\left(\frac{1}{n} - c\right)(n+1)\to0$.
So we know that:

$$
\begin{align}
  & \lim_{c\to0^+}\int_{c}^{1} f(x)\d{x} = \lim_{c\to0^+}\left(\left(\frac{1}{n} - c\right)(-1)^{n+1}(n+1) + \sum_{i=1}^{n-1}\frac{(-1)^{i+1}}{i}\right) \\
  \imply & \lim_{c\to0^+}\int_{c}^{1}f(x)\d{x} = \lim_{n\to\infty} \sum_{i=1}^{n-1}\frac{(-1)^{i+1}}{i} \\
  \imply & \lim_{c\to0^+}\int_{c}^{1}f(x)\d{x} = \sum_{i=1}^{\infty}\frac{(-1)^{i+1}}{i} \\
  \imply & \lim_{c\to0^+}\int_{c}^{1}f(x)\d{x} \text{ exists and is finite.}
\end{align}
$$

Now we have to show that this does *not* hold for $|f|$.
I will skip some of the intermediate computation and state that:

$$
\lim_{c\to0^+}\int_{c}^{1} |f(x)|\d{x} = \lim_{c\to0^+}\left(\left(\frac{1}{n} - c\right)(n+1) + \sum_{i=1}^{n-1}\frac{1}{i}\right)
$$

Since we already showed that as $n\to\infty$ (or $c\to0^+$), then $\left(\frac{1}{n} - c\right)(n+1)\to0$.
Therefore

$$
\begin{align}
  & \lim_{c\to0^+}\int_{c}^{1} |f(x)|\d{x} = \lim_{c\to0^+}\left(\left(\frac{1}{n} - c\right)(n+1) + \sum_{i=1}^{n-1}\frac{1}{i}\right) \\
  \imply & \lim_{c\to0^+}\int_{c}^{1} |f(x)|\d{x} = \lim_{n\to\infty} \sum_{i=1}^{n-1}\frac{1}{i} \\
  \imply & \lim_{c\to0^+}\int_{c}^{1} |f(x)|\d{x} = \sum_{i=1}^{\infty}\frac{1}{i}
\end{align}
$$

We know that $\sum_{i=1}^{\infty}\frac{1}{i}$ is the harmonic series, which diverges.
Therefore, it follows that $\lim_{c\to0^+}\int_{c}^{1} |f(x)|\d{x}$ diverges as well.
So I have constructed a function $f$ where:

- $\lim_{c\to0^+}\int_{c}^{1} f(x)\d{x}$ exists.
- $\lim_{c\to0^+}\int_{c}^{1} |f(x)|\d{x}$ does *not* exist.
