---
author:
  - John Lekberg <jclekberg@gmail.com>
date: 2016-02-23
...

\newcommand{\closed}[2]{\left[#1,#2\right]}
\newcommand{\open}[2]{\left(#1,#2\right)}
\newcommand{\openclosed}[2]{\left(#1,#2\right]}
\newcommand{\closedopen}[2]{\left[#1,#2\right)}
\renewcommand{\iff}{\Leftrightarrow\,}
\newcommand{\imply}{\Rightarrow\,}
\newcommand{\riemann}{\mathscr{R}}
\newcommand{\d}{\,\mathrm{d}}

# Statement

Suppose $f\in\riemann$ on $\closed{a}{b}$ for every $b > a$, where $a$ is fixed.
Define

$$
\int_{a}^{\infty}f(x)\d{x} = \lim_{b\to\infty}\int_{a}^{b}f(x)\d{x}
$$

if this limit exists (and is finite).
In that case, we say that the integral on the left *converges*.
If it also converges after $f$ has been replaced by $|f|$, it is said to converge *absolutely*.

Assume that $f(x) \geq 0$ and that $f$ decreases monotonically on $\closedopen{1}{\infty}$.
Prove that

$$
\int_{1}^{\infty}f(x)\d{x}
$$

converges if and only if

$$
\sum_{n=1}^{\infty}f(n)
$$

converges.
(This is the so-called "integral test" for convergence of series.)

# Solution

Theorem 6.12.c states:

> If $f\in\riemann(\alpha)$ on $\closed{a}{b}$ and if $a < c < b$, then $f\in\riemann(\alpha)$ on $\closed{a}{c}$ and on $\closed{c}{d}$, and
$$
\int_{a}^{c}f\d{\alpha} + \int_{c}^{b}f\d{\alpha} = \int_{a}^{b}f\d{\alpha}
$$s

This is useful, because for any $b\in\mathbb{N}$ where $b > 1$, then by Theorem 6.12.c:

$$
  \int_{1}^{b}f(x)\d{x} = \sum_{n=1}^{b}\int_{n}^{n+1}f(x)\d{x}
$$

Because $f$ decreases monotonically on $\closedopen{1}{\infty}$ we know that if $n \leq x \leq n+1$ then:

$$
\begin{align}
  & f(n+1) \leq f(x) \leq f(n) \\
  \imply & \int_{n}^{n+1} f(n+1) \d{x}\leq \int_{n}^{n+1}f(x)\d{x} \leq \int_{n}^{n+1} f(n)\d{x} \\
  \iff & f(n+1) \leq \int_{n}^{n+1} f(x) \d{x} \leq f(n) \\
  \imply & \sum_{n=1}^{b} f(n+1) \leq \sum_{n=1}^{b}\int_{n}^{n+1} f(x)\d{x} \leq \sum_{n=1}^{b} f(n) \\
  \iff & \sum_{n=1}^{b} f(n+1) \leq \int_{1}^{b} f(x)\d{x} \leq \sum_{n=1}^{b} f(n) \\
  \iff & (f(b+1) - f(1)) + \sum_{n=1}^{b}f(n) \leq \int_{1}^{b} f(x)\d{x} \leq \sum_{n=1}^{b} f(n)
\end{align}
$$

Because $f$ is monotonically decreasing on $\closedopen{1}{\infty}$ and because it is bounded below by $0$, then $\lim_{b\to\infty}f(b)$ exists.
Therefore:

$$
\lim_{b\to\infty}(f(b+1) - f(1))
$$

exists and is finite.
Let $\epsilon < 0$ be this limit.
Then it follows that:

$$
\begin{align}
  & (f(b+1) - f(1)) + \sum_{n=1}^{b}f(n) \leq \int_{1}^{b} f(x)\d{x} \leq \sum_{n=1}^{b} f(n) \\
  \imply & \lim_{b\to\infty}\left((f(b+1) - f(1)) + \sum_{n=1}^{b}f(n)\right) \leq \lim_{b\to\infty}\int_{1}^{b} f(x)\d{x} \leq \lim_{b\to\infty}\sum_{n=1}^{b} f(n) \\
  \iff & \epsilon + \sum_{n=1}^{\infty}f(n) \leq \int_{1}^{\infty}f(x)\d{x} \leq \sum_{n=1}^{\infty}f(n)
\end{align}
$$

From this it is clear that if $\sum_{n=1}^{\infty}f(n)$ converges then so does $\int_{1}^{\infty}f(x)\d{x}$, and if $\sum_{n=1}^{\infty}f(n)$ diverges then so does $\int_{1}^{\infty}f(x)\d{x}$.
Therefore:

$$
  \sum_{n=1}^{\infty}f(n)\text{ converges } \iff  \int_{1}^{\infty}f(x)\d{x}\text{ converges }
$$
